Add Identifiers, change ProgramType, proofs in progress

Strata/DL/Lambda/Identifiers.lean
@@ -5,11 +5,18 @@
 -/
 
 
-
+-- import Std.Data.HashMap.Lemmas
 import Strata.DL.Lambda.LTy
 import Strata.DL.Util.Map
 
 ---------------------------------------------------------------------
+
+-- -- Not merged in Lean release yet, so prove it ourselves
+@[simp]
+theorem Std.HashMap.contains_eq_false_iff_not_mem  {α : Type u} {β : Type v} [BEq α] [Hashable α] {m : Std.HashMap α β} {k : α} :
+m.contains k = false ↔ ¬k ∈ m := by
+  have m_cont := (Std.HashMap.contains_iff_mem (m:=m) (a:=k))
+  revert m_cont; cases (m.contains k) <;> simp
 
 namespace Lambda
 open Std (ToFormat Format format)
@@ -17,7 +24,7 @@ open Std (ToFormat Format format)
 section Identifiers
 
 /--
-Identifiers, optionally with their inferred monotype.
+Identifiers with a name and additional metadata
 -/
 structure Identifier (IDMeta : Type) : Type where
   name : String
@@ -33,6 +40,9 @@ instance : ToString (Identifier IDMeta) where
 instance {IDMeta} [Inhabited IDMeta] : Coe String (Identifier IDMeta) where
   coe s := ⟨s, Inhabited.default⟩
 
+/--
+Identifiers, optionally with their inferred monotype.
+-/
 abbrev IdentT (IDMeta : Type) := (Identifier IDMeta) × Option LMonoTy
 abbrev IdentTs (IDMeta : Type) := List (IdentT IDMeta)
 
@@ -52,6 +62,77 @@ def IdentTs.idents (xs : (IdentTs IDMeta)) : List (Identifier IDMeta) :=
 
 def IdentTs.monotys? (xs : (IdentTs IDMeta)) : List (Option LMonoTy) :=
   xs.map Prod.snd
+
+abbrev Identifiers IDMeta := Std.HashMap String IDMeta
+
+def Identifiers.default {IDMeta} : Identifiers IDMeta := Std.HashMap.emptyWithCapacity
+
+/-
+For an informative error message
+-/
+def Identifiers.addWithError {IDMeta} (m: Identifiers IDMeta) (x: Identifier IDMeta) (f: Format) : Except Format (Identifiers IDMeta) :=
+  let (b, m') := m.containsThenInsertIfNew x.name x.metadata
+  if b then .error f else .ok m'
+
+def Identifiers.add {IDMeta} (m: Identifiers IDMeta) (x: Identifier IDMeta) : Except Format (Identifiers IDMeta) :=
+  m.addWithError x f!"Error: duplicate identifier {x.name}"
+
+def Identifiers.contains {IDMeta} [DecidableEq IDMeta] (m: Identifiers IDMeta) (x: Identifier IDMeta) : Bool :=
+  match m[x.name]?with
+  | some i => x.metadata == i
+  | none => false
+
+theorem Identifiers.addWithErrorNotin {IDMeta} [DecidableEq IDMeta] {m m': Identifiers IDMeta} {x: Identifier IDMeta}: m.addWithError x f = .ok m' → m.contains x = false := by
+  unfold addWithError contains;
+  match h: (Std.HashMap.containsThenInsertIfNew m x.name x.metadata) with
+  | ⟨b, m'⟩ =>
+    simp;
+    cases b with
+    | true => simp
+    | false =>
+      simp; intro C; subst m';
+      have Hnotin := (Std.HashMap.containsThenInsertIfNew_fst (m:=m) (k:=x.name) (v:=x.metadata));
+      rw[h] at Hnotin;
+      symm at Hnotin
+      rw [Std.HashMap.contains_eq_isSome_getElem?] at Hnotin
+      revert Hnotin
+      cases m[x.name]? <;> simp
+
+
+
+-- Does this exist
+theorem not_false {P: Prop} [Decidable P]: ¬ P → (if P then x else y) = y :=
+  by grind
+
+theorem Identifiers.addWithErrorContains {IDMeta} [DecidableEq IDMeta] {m m': Identifiers IDMeta} {x: Identifier IDMeta}: m.addWithError x f = .ok m' → ∀ y, m'.contains y ↔ x = y ∨ m.contains y := by
+  unfold addWithError contains;
+  have m_contains := (Std.HashMap.containsThenInsertIfNew_fst (m:=m) (k:=x.name) (v:=x.metadata));
+  have m'_def := (Std.HashMap.containsThenInsertIfNew_snd (m:=m) (k:=x.name) (v:=x.metadata));
+  revert m_contains m'_def
+  rcases (Std.HashMap.containsThenInsertIfNew m x.name x.metadata) with ⟨b, m''⟩; simp; intros b_eq m''_eq; subst b m'';
+  cases m_contains: (Std.HashMap.contains m x.name) <;> simp; intros m'_eq; subst m'_eq; intros y; rw[Std.HashMap.getElem?_insertIfNew];
+  cases name_eq: (x.name == y.name)
+  case false =>
+    simp; intros x_eq_y; subst x; rw[BEq.rfl ] at name_eq; contradiction
+  case true =>
+    rw[beq_iff_eq] at name_eq
+    simp; rw[Std.HashMap.contains_eq_false_iff_not_mem] at m_contains;
+    -- is there a better way?
+    rw[not_false m_contains]; simp
+    cases meta_eq: (x.metadata == y.metadata)
+    case false => grind
+    case true =>
+      rw[beq_iff_eq] at meta_eq
+      constructor
+      . intros _; apply Or.inl; cases x; cases y; grind
+      . rw[meta_eq]; intros _; rfl
+
+def Identifiers.eq {IDMeta} (m1 m2: Identifiers IDMeta) : Prop :=
+  Std.HashMap.Equiv m1 m2
+
+instance [ToFormat IDMeta] : ToFormat (Identifiers IDMeta) where
+  format m := format (m.toList)
+
 
 ---------------------------------------------------------------------
 
